Allow a while loop with an ST effect

kremlib/C.Loops.fst
@@ -171,6 +171,24 @@ let rec while #test_pre #test_post test body =
     while #test_pre #test_post test body
   end
 
+(* Same while loop as before but this time using the ST effect *)
+val while_st:
+  #test_pre: (HS.mem -> GTot Type0) ->
+  #test_post: (bool -> HS.mem -> GTot Type0) ->
+  $test: (unit -> ST bool
+    (requires (fun h -> test_pre h))
+    (ensures (fun h0 x h1 -> test_post x h1))) ->
+  body: (unit -> ST unit
+    (requires (fun h -> test_post true h))
+    (ensures (fun h0 _ h1 -> test_pre h1))) ->
+  ST unit
+    (requires (fun h -> test_pre h))
+    (ensures (fun h0 _ h1 -> test_post false h1))
+let rec while_st #test_pre #test_post test body =
+  if test () then begin
+    body ();
+    while_st #test_pre #test_post test body
+  end
 
 (* To be extracted as:
     int i = <start>;
